7c, switch constraint systems to be a set of constraints

Deduction.thy
@@ -47,7 +47,7 @@ Constraint "msg list " "msg list " "msg " ( "((2_/|_)/} _) " [67,67,67]66)
 they are popped from the head of the first list and are push to the top
 of the second one *)
 
-type_synonym system = "constraint list"
+type_synonym system = "constraint set"
 
 (* (a) *)
 (* functions lifted to msg list get a postfix l
@@ -58,7 +58,8 @@ definition sapplyl::"subst_msg \<Rightarrow> msg list \<Rightarrow> msg list" wh
 definition sapplyc:: "subst_msg \<Rightarrow> constraint \<Rightarrow> constraint" where
 "sapplyc s c = (case c of  a|m}t \<Rightarrow> (sapplyl s a)|(sapplyl s m)}( sapply_msg s t))"
 definition sapplys:: "subst_msg \<Rightarrow> system \<Rightarrow> system" where
-"sapplys s cs = map (sapplyc s) cs"
+"sapplys s cs = image (sapplyc s) cs"
+
 
 lemma sapplyc_scomp:"sapplyc (scomp_msg t s) c = sapplyc t (sapplyc s (c))"
   apply(cases c)
@@ -71,7 +72,7 @@ definition fvl:: "msg list \<Rightarrow> var set" where
 definition fvc:: "constraint \<Rightarrow> var set" where
 "fvc c = (case c of a|m}t \<Rightarrow> (fvl a) \<union> (fvl m) \<union> (fv_msg t))"
 definition fvs:: "system \<Rightarrow> var set" where
-"fvs cs = (\<Union>c \<in> set cs. fvc c)"
+"fvs cs = (\<Union>c \<in> cs. fvc c)"
 
 (* (b) *)
 (* solution set *)
@@ -79,30 +80,55 @@ definition solved:: "constraint \<Rightarrow> bool" where
 "solved c = (case c of (m|a}t) \<Rightarrow> ((set m \<union> set a) \<turnstile> t))"
 
 definition sol:: "system \<Rightarrow> subst_msg set" where
-"sol cs = {s. (\<forall> c \<in> set cs. solved (sapplyc s c))}"
+"sol cs = {s. (\<forall> c \<in> cs. solved (sapplyc s c))}"
 
-lemma solE: "s \<in> sol cs \<Longrightarrow> ((\<And>c. c \<in> set cs \<Longrightarrow> solved (sapplyc s c)) \<Longrightarrow> P) \<Longrightarrow>P"
+lemma solE: "s \<in> sol cs \<Longrightarrow> ((\<And>c. c \<in> cs \<Longrightarrow> solved (sapplyc s c)) \<Longrightarrow> P) \<Longrightarrow>P"
   by(auto simp add:sol_def)
 
-lemma solI: "(\<And>c. c \<in> set cs \<Longrightarrow> solved (sapplyc s c)) \<Longrightarrow> s \<in> sol cs"
+lemma solI: "(\<And>c. c \<in> cs \<Longrightarrow> solved (sapplyc s c)) \<Longrightarrow> s \<in> sol cs"
   by(auto simp add:sol_def)
 
 (* lemmas *)
 
-lemma sol_concat: "sol(cs @ cs') = sol(cs) \<inter> sol(cs')"
+lemma sol_concat: "sol(cs \<union> cs') = sol(cs) \<inter> sol(cs')"
 proof((rule equalityI;rule subsetI),rule IntI)
 qed(auto simp add:sol_def)
 
 lemma "sol_scomp": "t \<in> sol(sapplys s cs) \<Longrightarrow> (scomp_msg t s) \<in> sol(cs)"
 proof(rule solI, erule solE)
   fix c
-  assume w:"c \<in> set cs"
-  assume x:"\<And>d. d \<in> set (sapplys s cs) \<Longrightarrow> solved (sapplyc t d)"
+  assume w:"c \<in> cs"
+  assume x:"\<And>d. d \<in> (sapplys s cs) \<Longrightarrow> solved (sapplyc t d)"
   have "solved (sapplyc (scomp_msg t s) c) = solved (sapplyc t (sapplyc s c))" (is "_ = solved (sapplyc t (?d))")
     by(simp add: sapplyc_scomp)
-  moreover have "?d \<in> set (sapplys s cs)" by(simp add:w sapplys_def)
+  moreover have "?d \<in> (sapplys s cs)" by(simp add:w sapplys_def)
   ultimately show "solved (sapplyc (scomp_msg t s) c)"
     by(simp add:x)
 qed
+
+(* (c) *)
+inductive rer1 :: "constraint \<Rightarrow> subst_msg \<Rightarrow> system \<Rightarrow> bool "
+("(_)/\<leadsto>1[_]/ (_)" [64,64,64]63)    where
+rer1_unify: "t\<noteq>Variable _ \<Longrightarrow> u \<in> set m \<union> set a \<Longrightarrow> unify_msg [(t,u)] = Some s \<Longrightarrow> (a|m}t)\<leadsto>1[s] {}"
+| rer1_comp_hash:"(a|m} (Hash t)) \<leadsto>1[(%x.(Variable x))] {(a|m} t)}"
+| rer1_comp_concat:"(a|m} (Concat t u)) \<leadsto>1[(%x.(Variable x))] {a|m} t, a|m} u}"
+| rer1_comp_sym_encrypt:"(a|m} (Sym_encrypt t u)) \<leadsto>1[(%x.(Variable x))] {a|m} t, a|m} u}"
+| rer1_comp_pub_encrypt:"(a|m} (Pub_encrypt t u)) \<leadsto>1[(%x.(Variable x))] {a|m} t, a|m} u}"
+| rer1_comp_sign:"(a|m} (Sign t (Const ''intruder''))) \<leadsto>1[(%x.(Variable x))] {a|m} t}"
+| rer1_proj: "((Concat u v)#a) | m } t \<leadsto>1[(%x. Variable x)] {((u#v#a) | ((Concat u v)#m) } t)}"
+| rer1_sdec: "((Sym_encrypt u k)#a) | m } t \<leadsto>1[(%x. Variable x)]
+ {  ((u#a) | ((Sym_encrypt u k)#m) } t) ,
+    (a | ((Sym_encrypt u k)#m) } k)     }"
+| rer1_adec: "((Pub_encrypt u (Variable ''intruder''))#a) | m } t \<leadsto>1[(%x. Variable x)]
+ { ((u#a) | ((Pub_encrypt u (Variable ''intruder''))#m) } t) }"
+| rer1_ksub: "x=Pub_encrypt u (Variable agent) \<Longrightarrow>
+s=(%v. Variable (if v=agent then ''intruder'' else v)) \<Longrightarrow>
+(x#a) | m } t  \<leadsto>1[s] { sapplyc s ((x#a) | m } t) }"
+
+inductive rer :: "system \<Rightarrow> subst_msg \<Rightarrow> system \<Rightarrow> bool " ("(_)/\<leadsto>[_]/ _ " [73,73,73]72) where
+"c \<leadsto>1[s] cs \<Longrightarrow> (insert c cs') \<leadsto>[s] (cs \<union> (sapplys s cs'))"
+
+definition rer_star :: "system \<Rightarrow>subst_msg \<Rightarrow> system \<Rightarrow> bool" ("(_)/\<leadsto>*[_]/ _ " [73,73,73]72) where
+"cs \<leadsto>*[s] cs' = ((cs, cs') \<in> (rtrancl { (x, y) . (x \<leadsto>[s] y) }))"
 
 end
